coq/set/Lang1/Semantics.v
@@ -40,43 +40,6 @@ Definition eval1 (e:Env) (p:Formula) (n:nat) (x:set) : Prop :=
 Definition eval2 (e:Env) (p:Formula) (n m:nat) (x y:set) : Prop :=
     eval (bind (bind e n x) m y) p.
 
-Lemma relevance : forall (e e':Env) (p:Formula), 
-    envEqualOn p e e' -> eval e p <-> eval e' p.
-Proof.
-    intros e e' p. unfold envEqualOn. revert e e'.
-    induction p as [|n m|p1 IH1 p2 IH2|n p1 IH1]; intros e e' H; simpl.
-    - tauto.
-    - split. 
-        + apply equal_lr; apply H.
-            { left. reflexivity. }
-            { right. left. reflexivity. }
-        + apply equal_lr; apply equalSym; apply H.
-            { left. reflexivity. }
-            { right. left. reflexivity. }
-    - rewrite (IH1 e e'), (IH2 e e').
-        + tauto.
-        + intros n H'. apply H. simpl. apply in_or_app. right. assumption.
-        + intros n H'. apply H. simpl. apply in_or_app. left.  assumption.
-    - split; intros H' x.
-        + rewrite (IH1 (bind e' n x) (bind e n x)). 
-            { apply H'. }
-            { intros m.  destruct (eq_nat_dec n m) as [E|E].
-                { subst. rewrite bindSame, bindSame. intros. apply equalRefl. }
-                { rewrite bindDiff, bindDiff.
-                    { intros H''. apply equalSym. apply H. simpl. 
-                      apply removeStill; assumption. }
-                    { assumption. }
-                    { assumption. }}}
-        + rewrite (IH1 (bind e n x) (bind e' n x)). 
-            { apply H'. }
-            { intros m H''. destruct (eq_nat_dec n m) as [E|E].
-                { subst. rewrite bindSame, bindSame. apply equalRefl. }
-                { rewrite bindDiff, bindDiff.
-                    { apply H. simpl. apply removeStill; assumption. }
-                    { assumption. }
-                    { assumption. }}}
-Qed.
-
 Lemma evalBot : forall (e:Env), eval e Bot <-> False.
 Proof. intros e. unfold eval. split; intros H; assumption. Qed.
 
@@ -233,20 +196,3 @@ Proof.
     - assumption.
 Qed.
 
-Lemma evalEnvEqual : forall (e e':Env) (p:Formula),
-    envEqual e e' -> eval e p <-> eval e' p.
-Proof.
-    intros e e' p H. apply relevance. intros n H'. apply H.
-Qed.
-
-
-Lemma evalNotInFree : forall (e:Env) (n:nat) (x:set) (p:Formula),
-    ~In n (free p) -> eval (bind e n x) p <-> eval e p.
-Proof.
-    intros e n x p H. apply relevance. intros m H'. 
-    destruct (eq_nat_dec n m) as [E|E].
-    - subst. apply H in H'. contradiction.
-    - rewrite bindDiff. 
-        + apply equalRefl.
-        + assumption.
-Qed.
